theories/Lambda/ExprCore.v
@@ -4,6 +4,7 @@ Require Import ExtLib.Core.RelDec.
 Require Import ExtLib.Data.List.
 Require Import ExtLib.Relations.TransitiveClosure.
 Require Import ExtLib.Recur.Relation.
+Require Import ExtLib.Tactics.Consider.
 
 Set Implicit Arguments.
 Set Strict Implicit.
@@ -53,6 +54,44 @@ Section env.
     eapply Fix. eapply wf_leftTrans. eapply wf_expr_acc.
     destruct x; auto.
   Qed.
+
+  Section sdec.
+    Variable RelDec_eq_typ : RelDec (@eq typ).
+    Variable func_eq : func -> func -> bool.
+
+    Fixpoint expr_eq_sdec (e1 e2 : expr) : bool :=
+      match e1 , e2 with
+      | Var v1 , Var v2 => EqNat.beq_nat v1 v2
+      | UVar v1 , UVar v2 => EqNat.beq_nat v1 v2
+      | Inj f1 , Inj f2 => func_eq f1 f2
+      | App f1 e1 , App f2 e2 =>
+        if expr_eq_sdec f1 f2 then
+          expr_eq_sdec e1 e2
+        else
+          false
+      | Abs t1 e1 , Abs t2 e2 =>
+        if t1 ?[ eq ] t2 then expr_eq_sdec e1 e2
+        else false
+      | _ , _ => false
+      end.
+
+    Variable RelDec_Correct_typ : RelDec_Correct RelDec_eq_typ.
+    Variable func_eq_ok : forall a b, func_eq a b = true -> a = b.
+
+    Theorem expr_eq_sdec_ok : forall e1 e2,
+        expr_eq_sdec e1 e2 = true ->
+        e1 = e2.
+    Proof.
+      induction e1; destruct e2; simpl; intros; try congruence.
+      { eapply EqNat.beq_nat_true in H. congruence. }
+      { eapply func_eq_ok in H. congruence. }
+      { apply Bool.andb_true_iff in H.
+        destruct H. eapply IHe1_1 in H. eapply IHe1_2 in H0. congruence. }
+      { consider (t ?[ eq ] t0).
+        intros. apply IHe1 in H0. congruence. }
+      { eapply EqNat.beq_nat_true in H. congruence. }
+    Qed.
+  End sdec.
 
   Variable RelDec_eq_typ : RelDec (@eq typ).
   Variable RelDec_eq_func : RelDec (@eq func).
